Try to fix proof

new/etc/update-goose-new.py
@@ -67,6 +67,9 @@ projs = [
             "github.com/prometheus/client_golang/prometheus",
             "go.etcd.io/etcd/server/v3/config",
             "go.etcd.io/etcd/server/v3/auth",
+            "go.opentelemetry.io/otel/trace",
+            "go.opentelemetry.io/otel/attribute",
+            "go.etcd.io/etcd/server/v3/features",
             # cindex:
             "go.etcd.io/etcd/server/v3/etcdserver/cindex",
             # Axiomatized for cindex:
